better names

src/theories/Reflection/FM.v
@@ -17,12 +17,12 @@ MetaCoq Quote Definition c_not := @not.
 MetaCoq Quote Definition c_or := @or.
 MetaCoq Quote Definition c_and := @and.
 
-Section ReflectFM.
+Section ExtractFM.
   Variable (s: signature).
   Variable (m: model s).
 
-  Variable (reflect_t2tm : forall c, term -> list (option ({srt & (tm s c srt)})) -> option ({srt & (tm s c srt)})).
-  Variable (reflect_ind2srt : inductive -> option (sig_sorts s)).
+  Variable (extract_t2tm : forall c, term -> list (option ({srt & (tm s c srt)})) -> option ({srt & (tm s c srt)})).
+  Variable (extract_ind2srt : inductive -> option (sig_sorts s)).
 
   Variable (sort_eq_dec: EquivDec.EqDec (sig_sorts s) eq).
 
@@ -38,7 +38,7 @@ Section ReflectFM.
       end;
     mk_var SLNil _ := None.
 
-  Fixpoint reflect_t2tm' (c: ctx s) (acc: nat) (t: term) : option ({srt & tm s c srt}) :=  
+  Fixpoint extract_t2tm' (c: ctx s) (acc: nat) (t: term) : option ({srt & tm s c srt}) :=  
     match t with 
     | tRel n => 
       match mk_var c (n - acc) with 
@@ -46,13 +46,13 @@ Section ReflectFM.
         Some (existT _ srt (TVar v))
       | None => None
       end
-    | tApp f es => reflect_t2tm c t (map (reflect_t2tm' c acc) es)
-    | _ => reflect_t2tm c t []
+    | tApp f es => extract_t2tm c t (map (extract_t2tm' c acc) es)
+    | _ => extract_t2tm c t []
     end.
 
   Obligation Tactic := intros.
-  Equations reflect_t2fm (c: ctx s) (anon_acc: nat) (t: term) : option (fm _ c) by struct t := 
-    reflect_t2fm c acc t := 
+  Equations extract_t2fm (c: ctx s) (anon_acc: nat) (t: term) : option (fm _ c) by struct t := 
+    extract_t2fm c acc t := 
       if eq_term t c_True then Some FTrue else 
       if eq_term t c_False then Some FFalse else
       match t with
@@ -60,7 +60,7 @@ Section ReflectFM.
         if eq_term f c_eq then 
           match es with 
           | _ :: tl :: tr :: _ => 
-            match reflect_t2tm' c acc tl, reflect_t2tm' c acc tr with 
+            match extract_t2tm' c acc tl, extract_t2tm' c acc tr with 
             | Some l, Some r => 
               let (sl, el) := l in 
               let (sr, er) := r in 
@@ -76,7 +76,7 @@ Section ReflectFM.
         else if eq_term f c_or then 
           match es with 
           | tl :: tr :: _ => 
-            match reflect_t2fm c acc tl, reflect_t2fm c acc tr with 
+            match extract_t2fm c acc tl, extract_t2fm c acc tr with 
             | Some l, Some r => Some (@FOr _ c l r)
             | _, _ => None
             end
@@ -85,7 +85,7 @@ Section ReflectFM.
         else if eq_term f c_and then 
           match es with 
           | tl :: tr :: _ => 
-            match reflect_t2fm c acc tl, reflect_t2fm c acc tr with 
+            match extract_t2fm c acc tl, extract_t2fm c acc tr with 
             | Some l, Some r => Some (@FAnd _ c l r)
             | _, _ => None
             end
@@ -94,7 +94,7 @@ Section ReflectFM.
         else if eq_term f c_not then 
           match es with 
           | x :: _ => 
-            match reflect_t2fm c acc x with 
+            match extract_t2fm c acc x with 
             | Some x' => Some (FNeg _ x')
             | None => None
             end
@@ -105,18 +105,18 @@ Section ReflectFM.
       | tProd ba_name pre pst => 
         match ba_name.(binder_name) with 
         | nAnon => 
-          match reflect_t2fm c acc pre, reflect_t2fm c (S acc) pst with 
+          match extract_t2fm c acc pre, extract_t2fm c (S acc) pst with 
           | Some el, Some er => Some (FImpl el er)
           | _, _ => None
           end
         | nNamed _ => 
           match pre with 
           | tInd i _ => 
-            let srt := reflect_ind2srt i in 
+            let srt := extract_ind2srt i in 
             match srt with 
             | Some srt => 
               let c' := Snoc _ c srt in
-              let inner := reflect_t2fm c' acc pst in 
+              let inner := extract_t2fm c' acc pst in 
               match inner with 
               | Some fm => Some (FForall _ fm)
               | None => None
@@ -130,7 +130,7 @@ Section ReflectFM.
       | _ => None
       end.
 
-  (* TODO: soundness lemma; forall c t fm, reflect_t2fm c t = Some fm -> (forall v, interp_coq_tm v t <-> interp_fm v fm) *)
+  (* TODO: soundness lemma; forall c t fm, extract_t2fm c t = Some fm -> (forall v, interp_coq_tm v t <-> interp_fm v fm) *)
 
   (* Some light tests *)
   (* Variable (c: ctx s).
@@ -142,18 +142,18 @@ Section ReflectFM.
   MetaCoq Quote Definition test_5 := (forall (x: unit), True).
   MetaCoq Quote Definition test_6 := (forall (x: unit), True \/ False \/ ~ True).
 
-  Eval vm_compute in reflect_t2fm c 0 test_1.
-  Eval vm_compute in reflect_t2fm c 0 test_2. 
-  Eval vm_compute in reflect_t2fm c 0 test_3.
-  Eval vm_compute in reflect_t2fm c 0 test_4.
-  Eval vm_compute in reflect_t2fm c 0 test_5.
-  Eval vm_compute in reflect_t2fm c 0 test_6. *)
-End ReflectFM.
+  Eval vm_compute in extract_t2fm c 0 test_1.
+  Eval vm_compute in extract_t2fm c 0 test_2. 
+  Eval vm_compute in extract_t2fm c 0 test_3.
+  Eval vm_compute in extract_t2fm c 0 test_4.
+  Eval vm_compute in extract_t2fm c 0 test_5.
+  Eval vm_compute in extract_t2fm c 0 test_6. *)
+End ExtractFM.
     
 
 
 
-Section ParseFM.
+Section ReifyFM.
   Variable (Ty: Type).
   Variable (interp_ty: Ty -> Type).
 
@@ -162,28 +162,28 @@ Section ParseFM.
   Notation res_ty := (option ({ty & interp_ty ty})).
   Notation env_ty := (snoc_list ({ty & interp_ty ty})).
 
-  Variable (parse_t2tm : term -> list res_ty -> res_ty).
-  Variable (parse_ind : inductive -> option Ty).
+  Variable (reify_t2tm : term -> list res_ty -> res_ty).
+  Variable (reify_ind : inductive -> option Ty).
 
-  Fixpoint parse_var (env: env_ty) (n: nat) : res_ty :=
+  Fixpoint reify_var (env: env_ty) (n: nat) : res_ty :=
     match env, n with 
     | Snoc _ x, 0 => Some x
-    | Snoc env' _, S n' => parse_var env' n'
+    | Snoc env' _, S n' => reify_var env' n'
     | SLNil, _ => None
     end.
 
-  Fixpoint parse_t2tm' (env: env_ty) (acc: nat) (t: term) : res_ty :=  
+  Fixpoint reify_t2tm' (env: env_ty) (acc: nat) (t: term) : res_ty :=  
     match t with 
-    | tRel n => parse_var env (n - acc)
-    | tApp f es => parse_t2tm t (map (parse_t2tm' env acc) es)
-    | _ => parse_t2tm t []
+    | tRel n => reify_var env (n - acc)
+    | tApp f es => reify_t2tm t (map (reify_t2tm' env acc) es)
+    | _ => reify_t2tm t []
     end.
 
   Definition ret (p: Prop) : option (env_ty -> option Prop) := Some (fun _ => Some p).
 
   Obligation Tactic := intros.
-  Equations parse_t2fm (env: env_ty) (anon_acc: nat) (t: term) : option Prop by struct t := 
-    parse_t2fm env acc t := 
+  Equations reify_t2fm (env: env_ty) (anon_acc: nat) (t: term) : option Prop by struct t := 
+    reify_t2fm env acc t := 
       if eq_term t c_True then Some True else 
       if eq_term t c_False then Some False else
       match t with
@@ -191,7 +191,7 @@ Section ParseFM.
         if eq_term f c_eq then 
           match es with 
           | _ :: tl :: tr :: _ => 
-            match parse_t2tm' env acc tl, parse_t2tm' env acc tr with 
+            match reify_t2tm' env acc tl, reify_t2tm' env acc tr with 
             | Some l, Some r => 
               let (tl, el) := l in 
               let (tr, er) := r in 
@@ -207,7 +207,7 @@ Section ParseFM.
         else if eq_term f c_or then 
           match es with 
           | tl :: tr :: _ => 
-            match parse_t2fm env acc tl, parse_t2fm env acc tr with 
+            match reify_t2fm env acc tl, reify_t2fm env acc tr with 
             | Some l, Some r => Some (l \/ r)
             | _, _ => None
             end
@@ -216,7 +216,7 @@ Section ParseFM.
         else if eq_term f c_and then 
           match es with 
           | tl :: tr :: _ => 
-            match parse_t2fm env acc tl, parse_t2fm env acc tr with 
+            match reify_t2fm env acc tl, reify_t2fm env acc tr with 
             | Some l, Some r => Some (l /\ r)
             | _, _ => None
             end
@@ -225,7 +225,7 @@ Section ParseFM.
         else if eq_term f c_not then 
           match es with 
           | x :: _ => 
-            match parse_t2fm env acc x with 
+            match reify_t2fm env acc x with 
             | Some x' => Some (~ x')
             | None => None
             end
@@ -236,20 +236,20 @@ Section ParseFM.
       | tProd ba_name pre pst => 
         match ba_name.(binder_name) with 
         | nAnon =>
-          match parse_t2fm env acc pre, parse_t2fm env (S acc) pst with 
+          match reify_t2fm env acc pre, reify_t2fm env (S acc) pst with 
           | Some el, Some er => Some (el -> er)
           | _, _ => None
           end
         | nNamed _ =>
           match pre with 
           | tInd i _ => 
-            let ty := parse_ind i in 
+            let ty := reify_ind i in 
             match ty with
             | Some ty' => Some (
               forall x: interp_ty ty', 
               exists p',
               let env' := Snoc _ env (existT _ ty' x) in
-                  parse_t2fm env' acc pst = Some p' /\
+                  reify_t2fm env' acc pst = Some p' /\
                   p'
               )
             | None => None
@@ -267,10 +267,10 @@ Section ParseFM.
   MetaCoq Quote Definition test_5 := (forall (x: unit), x = tt).
   MetaCoq Quote Definition test_6 := (forall (x: unit), True \/ False \/ ~ True).
 
-  Eval vm_compute in parse_t2fm (SLNil _)  0 test_1.
-  Eval vm_compute in parse_t2fm (SLNil _)  0 test_2. 
-  Eval vm_compute in parse_t2fm (SLNil _)  0 test_3.
-  Eval vm_compute in parse_t2fm (SLNil _)  0 test_4.
-  Eval vm_compute in parse_t2fm (SLNil _)  0 test_5.
-  Eval vm_compute in parse_t2fm (SLNil _)  0 test_6. *)
-End ParseFM.
+  Eval vm_compute in reify_t2fm (SLNil _)  0 test_1.
+  Eval vm_compute in reify_t2fm (SLNil _)  0 test_2. 
+  Eval vm_compute in reify_t2fm (SLNil _)  0 test_3.
+  Eval vm_compute in reify_t2fm (SLNil _)  0 test_4.
+  Eval vm_compute in reify_t2fm (SLNil _)  0 test_5.
+  Eval vm_compute in reify_t2fm (SLNil _)  0 test_6. *)
+End ReifyFM.
